src/HOL/Hoare/Separation.thy
@@ -1,0 +1,90 @@
+theory Separation = HoareAbort:
+
+types heap = "(nat \<Rightarrow> nat option)"
+
+
+text{* The semantic definition of a few connectives: *}
+
+constdefs
+ R:: "heap \<Rightarrow> heap \<Rightarrow> heap \<Rightarrow> bool"
+"R h h1 h2 == dom h1 \<inter> dom h2 = {} \<and> h = h1 ++ h2"
+
+ star:: "(heap \<Rightarrow> bool) \<Rightarrow> (heap \<Rightarrow> bool) \<Rightarrow> (heap \<Rightarrow> bool)"
+"star P Q == \<lambda>h. \<exists>h1 h2. R h h1 h2 \<and> P h1 \<and> Q h2"
+
+ singl:: "heap \<Rightarrow> nat \<Rightarrow> nat \<Rightarrow> bool"
+"singl h x y == dom h = {x} & h x = Some y"
+
+lemma "VARS x y z w h
+ {star (%h. singl h x y) (%h. singl h z w) h}
+ SKIP
+ {x \<noteq> z}"
+apply vcg
+apply(auto simp:star_def R_def singl_def)
+done
+
+text{* To suppress the heap parameter of the connectives, we assume it
+is always called H and add/remove it upon parsing/printing. Thus
+every pointer program needs to have a program variable H, and
+assertions should not contain any locally bound Hs - otherwise they
+may bind the implicit H. *}
+
+text{* Nice input syntax: *}
+
+syntax
+ "@singl" :: "nat \<Rightarrow> nat \<Rightarrow> bool" ("[_ \<mapsto> _]")
+ "@star" :: "bool \<Rightarrow> bool \<Rightarrow> bool" (infixl "**" 60)
+
+ML{*
+fun singl_tr [p,q] = Syntax.const "singl" $ Syntax.free "H" $ p $ q
+  | singl_tr ts = raise TERM ("singl_tr", ts);
+fun star_tr [P,Q] = Syntax.const "star" $
+      absfree("H",dummyT,P) $ absfree("H",dummyT,Q) $ Syntax.free "H"
+  | star_tr ts = raise TERM ("star_tr", ts);
+*}
+
+parse_translation {* [("@singl", singl_tr),("@star", star_tr)] *}
+
+lemma "VARS H x y z w
+ {[x\<mapsto>y] ** [z\<mapsto>w]}
+ SKIP
+ {x \<noteq> z}"
+apply vcg
+apply(auto simp:star_def R_def singl_def)
+done
+
+text{* Nice output syntax: *}
+
+ML{*
+fun singl_tr' [_,p,q] = Syntax.const "@singl" $ p $ q
+fun star_tr' [Abs(_,_,P),Abs(_,_,Q),_] = Syntax.const "@star" $ P $ Q
+*}
+
+print_translation {* [("singl", singl_tr'),("star", star_tr')] *}
+
+lemma "VARS H x y z w
+ {[x\<mapsto>y] ** [z\<mapsto>w]}
+ SKIP
+ {x \<noteq> z}"
+apply vcg
+apply(auto simp:star_def R_def singl_def)
+done
+
+
+consts llist :: "(heap * nat)set"
+inductive llist
+intros
+empty: "(%n. None, 0) : llist"
+cons: "\<lbrakk> R h h1 h2; pto h1 p q; (h2,q):llist \<rbrakk> \<Longrightarrow> (h,p):llist"
+
+lemma "VARS p q h
+ {(h,p) : llist}
+ h := h(q \<mapsto> p)
+ {(h,q) : llist}"
+apply vcg
+apply(rule_tac "h1.0" = "%n. if n=q then Some p else None" in llist.cons)
+prefer 3 apply assumption
+prefer 2 apply(simp add:singl_def dom_def)
+apply(simp add:R_def dom_def)
+
+
